<?xml version="1.0"?>


<!DOCTYPE rdf:RDF [
    <!ENTITY dcterms "http://purl.org/dc/terms/" >
    <!ENTITY owl "http://www.w3.org/2002/07/owl#" >
    <!ENTITY dc "http://purl.org/dc/elements/1.1/" >
    <!ENTITY xsd "http://www.w3.org/2001/XMLSchema#" >
    <!ENTITY skos "http://www.w3.org/2004/02/skos/core#" >
    <!ENTITY rdfs "http://www.w3.org/2000/01/rdf-schema#" >
    <!ENTITY rdf "http://www.w3.org/1999/02/22-rdf-syntax-ns#" >
]>


<rdf:RDF xmlns="http://mdr.semic.eu/def#"
     xml:base="http://mdr.semic.eu/def"
     xmlns:dc="http://purl.org/dc/elements/1.1/"
     xmlns:rdfs="http://www.w3.org/2000/01/rdf-schema#"
     xmlns:owl="http://www.w3.org/2002/07/owl#"
     xmlns:xsd="http://www.w3.org/2001/XMLSchema#"
     xmlns:rdf="http://www.w3.org/1999/02/22-rdf-syntax-ns#"
     xmlns:skos="http://www.w3.org/2004/02/skos/core#"
     xmlns:dcterms="http://purl.org/dc/terms/">
    <owl:Ontology rdf:about="http://mdr.testproject.eu/def">
        <rdfs:comment>The Metadata Registry Ontology is an implementation of the ISO 11179-3 meta-model for describing data elements.</rdfs:comment>
        <dc:title>Metadata Registry Ontology</dc:title>
        <owl:imports rdf:resource="http://www.w3.org/2004/02/skos/core"/>
    </owl:Ontology>
    


    <!-- 
    ///////////////////////////////////////////////////////////////////////////////////////
    //
    // Annotation properties
    //
    ///////////////////////////////////////////////////////////////////////////////////////
     -->

    


    <!-- http://purl.org/dc/elements/1.1/title -->

    <owl:AnnotationProperty rdf:about="&dc;title"/>
    


    <!-- 
    ///////////////////////////////////////////////////////////////////////////////////////
    //
    // Object Properties
    //
    ///////////////////////////////////////////////////////////////////////////////////////
     -->

    


    <!-- http://mdr.testproject.eu/def#affects -->

    <owl:ObjectProperty rdf:about="http://mdr.testproject.eu/def#affects">
        <rdfs:label>affects</rdfs:label>
        <rdfs:comment>States that the business rule affects (defines or constraints) a data element concept.</rdfs:comment>
        <rdfs:domain rdf:resource="http://mdr.testproject.eu/def#BusinessRule"/>
        <rdfs:range rdf:resource="http://mdr.testproject.eu/def#DataElementConcept"/>
    </owl:ObjectProperty>
    


    <!-- http://mdr.testproject.eu/def#conceptualDomain -->

    <owl:ObjectProperty rdf:about="http://mdr.testproject.eu/def#conceptualDomain">
        <rdfs:label>has conceptual domain</rdfs:label>
        <rdfs:comment>The Conceptual Domain of the Data Element Concept.</rdfs:comment>
        <rdfs:range rdf:resource="http://mdr.testproject.eu/def#ConceptualDomain"/>
        <rdfs:domain rdf:resource="http://mdr.testproject.eu/def#DataElementConcept"/>
    </owl:ObjectProperty>
    


    <!-- http://mdr.testproject.eu/def#contains -->

    <owl:ObjectProperty rdf:about="http://mdr.testproject.eu/def#contains">
        <rdfs:label>contains</rdfs:label>
        <rdfs:comment>A Value Meaning or Permissible Value contained respectively in a Enumerated Conceptual Domain or Enumerated Value Domain.</rdfs:comment>
    </owl:ObjectProperty>
    


    <!-- http://mdr.testproject.eu/def#context -->

    <owl:ObjectProperty rdf:about="http://mdr.testproject.eu/def#context">
        <rdfs:label>has context</rdfs:label>
        <rdfs:comment>The context of the element.</rdfs:comment>
        <rdfs:range rdf:resource="http://mdr.testproject.eu/def#Context"/>
    </owl:ObjectProperty>
    


    <!-- http://mdr.testproject.eu/def#datatype -->

    <owl:ObjectProperty rdf:about="http://mdr.testproject.eu/def#datatype">
        <rdfs:label>has datatype</rdfs:label>
        <rdfs:comment>The datatype of the Value Domain, i.e., the set of distinct values, characterized by properties of those values and by operations on those values.</rdfs:comment>
        <rdfs:domain rdf:resource="http://mdr.testproject.eu/def#ValueDomain"/>
    </owl:ObjectProperty>
    


    <!-- http://mdr.testproject.eu/def#expresses -->

    <owl:ObjectProperty rdf:about="http://mdr.testproject.eu/def#expresses">
        <rdfs:label>expresses</rdfs:label>
        <rdfs:comment>The Data Element Concept that is expressed by the Data Element.</rdfs:comment>
        <rdfs:domain rdf:resource="http://mdr.testproject.eu/def#DataElement"/>
        <rdfs:range rdf:resource="http://mdr.testproject.eu/def#DataElementConcept"/>
    </owl:ObjectProperty>
    


    <!-- http://mdr.testproject.eu/def#implements -->

    <owl:ObjectProperty rdf:about="http://mdr.testproject.eu/def#implements">
        <rdfs:label>implements</rdfs:label>
        <rdfs:comment>States that a high-level requirement (partially) implements a goal, or that a data element concept or business rule (partially) implements a high-level requirement.</rdfs:comment>
    </owl:ObjectProperty>
    


    <!-- http://mdr.testproject.eu/def#meaning -->

    <owl:ObjectProperty rdf:about="http://mdr.testproject.eu/def#meaning">
        <rdfs:label>has meaning</rdfs:label>
        <rdfs:comment>The Value Meaning of the Permissible Value.</rdfs:comment>
        <rdfs:domain rdf:resource="http://mdr.testproject.eu/def#PermissibleValue"/>
        <rdfs:range rdf:resource="http://mdr.testproject.eu/def#ValueMeaning"/>
    </owl:ObjectProperty>
    


    <!-- http://mdr.testproject.eu/def#objectClass -->

    <owl:ObjectProperty rdf:about="http://mdr.testproject.eu/def#objectClass">
        <rdfs:label>object class</rdfs:label>
        <rdfs:comment>The Object Class of the Data Element Concept.</rdfs:comment>
        <rdfs:domain rdf:resource="http://mdr.testproject.eu/def#DataElementConcept"/>
        <rdfs:range rdf:resource="http://mdr.testproject.eu/def#ObjectClass"/>
    </owl:ObjectProperty>
    


    <!-- http://mdr.testproject.eu/def#property -->

    <owl:ObjectProperty rdf:about="http://mdr.testproject.eu/def#property">
        <rdfs:label>has property</rdfs:label>
        <rdfs:comment>The Property of the Data Element Concept.</rdfs:comment>
        <rdfs:domain rdf:resource="http://mdr.testproject.eu/def#DataElementConcept"/>
        <rdfs:range rdf:resource="http://mdr.testproject.eu/def#Property"/>
    </owl:ObjectProperty>
    


    <!-- http://mdr.testproject.eu/def#representedBy -->

    <owl:ObjectProperty rdf:about="http://mdr.testproject.eu/def#representedBy">
        <rdfs:label>is represented by</rdfs:label>
        <rdfs:comment>The Value Domain that represents the Data Element.</rdfs:comment>
        <rdfs:domain rdf:resource="http://mdr.testproject.eu/def#DataElement"/>
        <rdfs:range rdf:resource="http://mdr.testproject.eu/def#ValueDomain"/>
    </owl:ObjectProperty>
    


    <!-- http://mdr.testproject.eu/def#represents -->

    <owl:ObjectProperty rdf:about="http://mdr.testproject.eu/def#represents">
        <rdfs:label>represents</rdfs:label>
        <rdfs:comment>The Conceptual Domain that is represented by the Value Domain.</rdfs:comment>
        <rdfs:range rdf:resource="http://mdr.testproject.eu/def#ConceptualDomain"/>
        <rdfs:domain rdf:resource="http://mdr.testproject.eu/def#ValueDomain"/>
    </owl:ObjectProperty>
    


    <!-- 
    ///////////////////////////////////////////////////////////////////////////////////////
    //
    // Data properties
    //
    ///////////////////////////////////////////////////////////////////////////////////////
     -->

    


    <!-- http://mdr.testproject.eu/def#rationale -->

    <owl:DatatypeProperty rdf:about="http://mdr.testproject.eu/def#rationale">
        <rdfs:label>rationale</rdfs:label>
        <rdfs:comment>The rationale of a requirement.</rdfs:comment>
        <rdfs:domain rdf:resource="http://mdr.testproject.eu/def#Requirement"/>
    </owl:DatatypeProperty>
    


    <!-- http://mdr.testproject.eu/def#value -->

    <owl:DatatypeProperty rdf:about="http://mdr.testproject.eu/def#value">
        <rdfs:label>has value</rdfs:label>
        <rdfs:comment>The concrete representation of the Permissible Value.</rdfs:comment>
        <rdfs:domain rdf:resource="http://mdr.testproject.eu/def#PermissibleValue"/>
    </owl:DatatypeProperty>
    


    <!-- 
    ///////////////////////////////////////////////////////////////////////////////////////
    //
    // Classes
    //
    ///////////////////////////////////////////////////////////////////////////////////////
     -->

    


    <!-- http://mdr.testproject.eu/def#BusinessRule -->

    <owl:Class rdf:about="http://mdr.testproject.eu/def#BusinessRule">
        <rdfs:label>Business Rule</rdfs:label>
        <rdfs:comment>Statement that defines or constrains some aspect of the e-Document.</rdfs:comment>
    </owl:Class>
    


    <!-- http://mdr.testproject.eu/def#ConceptualDomain -->

    <owl:Class rdf:about="http://mdr.testproject.eu/def#ConceptualDomain">
        <rdfs:label>Conceptual Domain</rdfs:label>
        <rdfs:comment>A set of valid Value Meanings.</rdfs:comment>
    </owl:Class>
    


    <!-- http://mdr.testproject.eu/def#Context -->

    <owl:Class rdf:about="http://mdr.testproject.eu/def#Context">
        <rdfs:label>Context</rdfs:label>
        <rdfs:comment>Universe of discourse.</rdfs:comment>
    </owl:Class>
    


    <!-- http://mdr.testproject.eu/def#DataElement -->

    <owl:Class rdf:about="http://mdr.testproject.eu/def#DataElement">
        <rdfs:label>Data Element</rdfs:label>
        <rdfs:subClassOf>
            <owl:Restriction>
                <owl:onProperty rdf:resource="http://mdr.testproject.eu/def#expresses"/>
                <owl:cardinality rdf:datatype="&xsd;nonNegativeInteger">1</owl:cardinality>
            </owl:Restriction>
        </rdfs:subClassOf>
        <rdfs:subClassOf>
            <owl:Restriction>
                <owl:onProperty rdf:resource="http://mdr.testproject.eu/def#representedBy"/>
                <owl:cardinality rdf:datatype="&xsd;nonNegativeInteger">1</owl:cardinality>
            </owl:Restriction>
        </rdfs:subClassOf>
        <rdfs:comment>A unit of data for which the definition, identification, representation and Permissible Values are specified by means of a set of attributes.</rdfs:comment>
    </owl:Class>
    


    <!-- http://mdr.testproject.eu/def#DataElementConcept -->

    <owl:Class rdf:about="http://mdr.testproject.eu/def#DataElementConcept">
        <rdfs:label>Data Element Concept</rdfs:label>
        <rdfs:subClassOf>
            <owl:Restriction>
                <owl:onProperty rdf:resource="http://mdr.testproject.eu/def#property"/>
                <owl:cardinality rdf:datatype="&xsd;nonNegativeInteger">1</owl:cardinality>
            </owl:Restriction>
        </rdfs:subClassOf>
        <rdfs:subClassOf>
            <owl:Restriction>
                <owl:onProperty rdf:resource="http://mdr.testproject.eu/def#conceptualDomain"/>
                <owl:cardinality rdf:datatype="&xsd;nonNegativeInteger">1</owl:cardinality>
            </owl:Restriction>
        </rdfs:subClassOf>
        <rdfs:subClassOf>
            <owl:Restriction>
                <owl:onProperty rdf:resource="http://mdr.testproject.eu/def#objectClass"/>
                <owl:cardinality rdf:datatype="&xsd;nonNegativeInteger">1</owl:cardinality>
            </owl:Restriction>
        </rdfs:subClassOf>
        <rdfs:comment>A concept that can be represented in the form of a Data Element, described independently of any particular representation.</rdfs:comment>
    </owl:Class>
    


    <!-- http://mdr.testproject.eu/def#EnumeratedConceptualDomain -->

    <owl:Class rdf:about="http://mdr.testproject.eu/def#EnumeratedConceptualDomain">
        <rdfs:label>Enumerated Conceptual Domain</rdfs:label>
        <rdfs:subClassOf rdf:resource="http://mdr.testproject.eu/def#ConceptualDomain"/>
        <rdfs:subClassOf>
            <owl:Restriction>
                <owl:onProperty rdf:resource="http://mdr.testproject.eu/def#contains"/>
                <owl:someValuesFrom rdf:resource="http://mdr.testproject.eu/def#ValueMeaning"/>
            </owl:Restriction>
        </rdfs:subClassOf>
        <rdfs:comment>A Conceptual Domain that is specified by a list of all its Value Meanings.</rdfs:comment>
    </owl:Class>
    


    <!-- http://mdr.testproject.eu/def#EnumeratedValueDomain -->

    <owl:Class rdf:about="http://mdr.testproject.eu/def#EnumeratedValueDomain">
        <rdfs:label>Enumerated Value Domain</rdfs:label>
        <rdfs:subClassOf rdf:resource="http://mdr.testproject.eu/def#ValueDomain"/>
        <rdfs:subClassOf>
            <owl:Restriction>
                <owl:onProperty rdf:resource="http://mdr.testproject.eu/def#contains"/>
                <owl:someValuesFrom rdf:resource="http://mdr.testproject.eu/def#PermissibleValue"/>
            </owl:Restriction>
        </rdfs:subClassOf>
        <rdfs:comment>A Value Domain that is specified by a list of all its Permissible Values.</rdfs:comment>
    </owl:Class>
    


    <!-- http://mdr.testproject.eu/def#Format -->

    <owl:Class rdf:about="http://mdr.testproject.eu/def#Format">
        <rdfs:label>e-Document Format</rdfs:label>
        <rdfs:subClassOf rdf:resource="http://mdr.testproject.eu/def#Context"/>
        <rdfs:comment>An e-Document format.</rdfs:comment>
    </owl:Class>
    


    <!-- http://mdr.testproject.eu/def#Goal -->

    <owl:Class rdf:about="http://mdr.testproject.eu/def#Goal">
        <rdfs:label>Goal</rdfs:label>
        <rdfs:comment>A goal that has to be achieved with the exchange of e-Documents.</rdfs:comment>
    </owl:Class>
    


    <!-- http://mdr.testproject.eu/def#Library -->

    <owl:Class rdf:about="http://mdr.testproject.eu/def#Library">
        <rdfs:label>Library of data elements</rdfs:label>
        <rdfs:subClassOf rdf:resource="http://mdr.testproject.eu/def#Context"/>
        <rdfs:comment>A library of data elements.</rdfs:comment>
    </owl:Class>
    


    <!-- http://mdr.testproject.eu/def#NonEnumeratedConceptualDomain -->

    <owl:Class rdf:about="http://mdr.testproject.eu/def#NonEnumeratedConceptualDomain">
        <rdfs:label>Non-Enumerated Conceptual Domain</rdfs:label>
        <rdfs:subClassOf rdf:resource="http://mdr.testproject.eu/def#ConceptualDomain"/>
        <rdfs:comment>A Conceptual Domain that is specified by a description rather than a list of all valid Value Meanings.</rdfs:comment>
    </owl:Class>
    


    <!-- http://mdr.testproject.eu/def#NonEnumeratedValueDomain -->

    <owl:Class rdf:about="http://mdr.testproject.eu/def#NonEnumeratedValueDomain">
        <rdfs:label>Non-Enumerated Value Domain</rdfs:label>
        <rdfs:subClassOf rdf:resource="http://mdr.testproject.eu/def#ValueDomain"/>
        <rdfs:comment>A Value Domain that is specified by a description rather than a list of all Permissible Values.</rdfs:comment>
    </owl:Class>
    


    <!-- http://mdr.testproject.eu/def#ObjectClass -->

    <owl:Class rdf:about="http://mdr.testproject.eu/def#ObjectClass">
        <rdfs:label>Object Class</rdfs:label>
        <rdfs:subClassOf rdf:resource="http://mdr.testproject.eu/def#NonEnumeratedConceptualDomain"/>
        <rdfs:comment>A set of ideas, abstractions, or things in the real world that are identified with explicit boundaries and meaning and whose properties and behaviour follow the same rules.</rdfs:comment>
    </owl:Class>
    


    <!-- http://mdr.testproject.eu/def#PermissibleValue -->

    <owl:Class rdf:about="http://mdr.testproject.eu/def#PermissibleValue">
        <rdfs:label>Permissible Value</rdfs:label>
        <rdfs:subClassOf>
            <owl:Restriction>
                <owl:onProperty rdf:resource="http://mdr.testproject.eu/def#value"/>
                <owl:cardinality rdf:datatype="&xsd;nonNegativeInteger">1</owl:cardinality>
            </owl:Restriction>
        </rdfs:subClassOf>
        <rdfs:subClassOf>
            <owl:Restriction>
                <owl:onProperty rdf:resource="http://mdr.testproject.eu/def#meaning"/>
                <owl:cardinality rdf:datatype="&xsd;nonNegativeInteger">1</owl:cardinality>
            </owl:Restriction>
        </rdfs:subClassOf>
        <rdfs:comment>An expression of a Value Meaning allowed in a specific Value Domain.</rdfs:comment>
    </owl:Class>
    


    <!-- http://mdr.testproject.eu/def#Property -->

    <owl:Class rdf:about="http://mdr.testproject.eu/def#Property">
        <rdfs:label>Property</rdfs:label>
        <rdfs:comment>A characteristic common to all members of an Object Class.</rdfs:comment>
    </owl:Class>
    


    <!-- http://mdr.testproject.eu/def#Requirement -->

    <owl:Class rdf:about="http://mdr.testproject.eu/def#Requirement">
        <rdfs:label>High-level Requirement</rdfs:label>
        <rdfs:comment>A high-level requirement that the e-Document format must fulfill.</rdfs:comment>
    </owl:Class>
    


    <!-- http://mdr.testproject.eu/def#ValueDomain -->

    <owl:Class rdf:about="http://mdr.testproject.eu/def#ValueDomain">
        <rdfs:label>Value Domain</rdfs:label>
        <rdfs:subClassOf>
            <owl:Restriction>
                <owl:onProperty rdf:resource="http://mdr.testproject.eu/def#represents"/>
                <owl:cardinality rdf:datatype="&xsd;nonNegativeInteger">1</owl:cardinality>
            </owl:Restriction>
        </rdfs:subClassOf>
        <rdfs:comment>A set of Permissible Values.</rdfs:comment>
    </owl:Class>
    


    <!-- http://mdr.testproject.eu/def#ValueMeaning -->

    <owl:Class rdf:about="http://mdr.testproject.eu/def#ValueMeaning">
        <rdfs:label>Value Meaning</rdfs:label>
        <rdfs:comment>The meaning or semantic content of a Value.</rdfs:comment>
    </owl:Class>
</rdf:RDF>



<!-- Generated by the OWL API (version 3.4.2) http://owlapi.sourceforge.net -->

